two things: combined leak_ext with ext_spec. made compiler noex build.

compiler/src/compiler/FlatImpUniqueSepLog.v
@@ -38,7 +38,7 @@ Module exec.
     Local Notation metrics := MetricLog.
 
     (* COQBUG(unification finds Type instead of Prop and fails to downgrade *)
-    Implicit Types post : trace -> mem -> locals -> metrics -> Prop.
+    Implicit Types post : trace -> io_trace -> mem -> locals -> metrics -> Prop.
 
     Definition lookup_op_locals (l: locals) (o: operand) :=
       match o with
@@ -48,131 +48,131 @@ Module exec.
 
     Inductive exec:
       stmt varname ->
-      trace -> mem -> locals -> metrics ->
-      (trace -> mem -> locals -> metrics -> Prop)
+      trace -> io_trace -> mem -> locals -> metrics ->
+      (trace -> io_trace -> mem -> locals -> metrics -> Prop)
     -> Prop :=
 
-    | interact: forall t m Keep mGive l mc action argvars argvals resvars outcome post,
+    | interact: forall k t m Keep mGive l mc action argvars argvals resvars outcome post,
         (Keep \*/ Some mGive) = Some m ->
         map.getmany_of_list l argvars = Some argvals ->
         ext_spec t mGive action argvals outcome ->
-        (forall mReceive resvals,
-            outcome mReceive resvals ->
+        (forall mReceive resvals klist,
+            outcome mReceive resvals klist ->
             exists l', map.putmany_of_list_zip resvars resvals l = Some l' /\
             forall m', (Keep \*/ Some mReceive) = Some m' ->
-            post (((mGive, action, argvals), (mReceive, resvals)) :: t) m' l'
+            post (leak_list klist :: k) (((mGive, action, argvals), (mReceive, resvals)) :: t) m' l'
                  (addMetricInstructions 1
                  (addMetricStores 1
                  (addMetricLoads 2 mc)))) ->
-        exec (SInteract resvars action argvars) t m l mc post
+        exec (SInteract resvars action argvars) k t m l mc post
 
-    | call: forall t m l mc binds fname args params rets fbody argvs st0 post outcome,
+    | call: forall k t m l mc binds fname args params rets fbody argvs st0 post outcome,
         map.get e fname = Some (params, rets, fbody) ->
         map.getmany_of_list l args = Some argvs ->
         map.putmany_of_list_zip params argvs map.empty = Some st0 ->
-        exec fbody t m st0 mc outcome ->
-        (forall t' m' mc' st1,
-            outcome t' m' st1 mc' ->
+        exec fbody (leak_unit :: k) t m st0 mc outcome ->
+        (forall k' t' m' mc' st1,
+            outcome k' t' m' st1 mc' ->
             exists retvs l',
               map.getmany_of_list st1 rets = Some retvs /\
               map.putmany_of_list_zip binds retvs l = Some l' /\
-              post t' m' l' mc') ->
-        exec (SCall binds fname args) t m l mc post
+              post k' t' m' l' mc') ->
+        exec (SCall binds fname args) k t m l mc post
 
-    | load: forall t m l mc sz R x a o v addr post,
+    | load: forall k t m l mc sz R x a o v addr post,
         map.get l a = Some addr ->
         R \*/ one sz (word.add addr (word.of_Z o)) v = Some m ->
-        post t m (map.put l x v)
+        post (leak_word (word.add addr (word.of_Z o)) :: k) t m (map.put l x v)
              (addMetricLoads 2
              (addMetricInstructions 1 mc)) ->
-        exec (SLoad sz x a o) t m l mc post
+        exec (SLoad sz x a o) k t m l mc post
 
-    | store: forall t m mc l sz a o addr v old_val val R post,
+    | store: forall k t m mc l sz a o addr v old_val val R post,
         map.get l a = Some addr ->
         map.get l v = Some val ->
         R \*/ one sz (word.add addr (word.of_Z o)) old_val = Some m ->
-        post t (mmap.force (R \*/ one sz (word.add addr (word.of_Z o)) val)) l
+        post (leak_word (word.add addr (word.of_Z o)) :: k) t (mmap.force (R \*/ one sz (word.add addr (word.of_Z o)) val)) l
              (addMetricLoads 1
              (addMetricInstructions 1
              (addMetricStores 1 mc))) ->
-        exec (SStore sz a v o) t m l mc post
+        exec (SStore sz a v o) k t m l mc post
 
-    | stackalloc: forall t mSmall l mc x n body post,
+    | stackalloc: forall k t mSmall l mc x n body post,
         n mod (bytes_per_word width) = 0 ->
         (forall (a: word) (oldstackbytes: tuple byte (Z.to_nat n)) (mCombined: mem),
             bytes a oldstackbytes \*/ Some mSmall = Some mCombined ->
-            exec body t mCombined (map.put l x a) (addMetricLoads 1 (addMetricInstructions 1 mc))
-                 (fun t' mCombined' l' mc' =>
+            exec body (consume_word a :: k) t mCombined (map.put l x a) (addMetricLoads 1 (addMetricInstructions 1 mc))
+                 (fun k' t' mCombined' l' mc' =>
                     exists (mSmall': mem) (newstackbytes: tuple byte (Z.to_nat n)),
                       Some mSmall' \*/ bytes a newstackbytes = Some mCombined' /\
-                      post t' mSmall' l' mc')) ->
-        exec (SStackalloc x n body) t mSmall l mc post
+                      post k' t' mSmall' l' mc')) ->
+        exec (SStackalloc x n body) k t mSmall l mc post
 
-    | lit: forall t m l mc x v post,
-        post t m (map.put l x (word.of_Z v))
+    | lit: forall k t m l mc x v post,
+        post k t m (map.put l x (word.of_Z v))
              (addMetricLoads 8
              (addMetricInstructions 8 mc)) ->
-        exec (SLit x v) t m l mc post
-    | op: forall t m l mc x op y y' z z' post,
+        exec (SLit x v) k t m l mc post
+    | op: forall k t m l mc x op y y' z z' post,
         map.get l y = Some y' ->
         lookup_op_locals l z = Some z' ->
-        post t m (map.put l x (interp_binop op y' z'))
+        post (leak_binop op y' z' ++ k) t m (map.put l x (interp_binop op y' z'))
              (addMetricLoads 2
              (addMetricInstructions 2 mc)) ->
-        exec (SOp x op y z) t m l mc post
-    | set: forall t m l mc x y y' post,
+        exec (SOp x op y z) k t m l mc post
+    | set: forall k t m l mc x y y' post,
         map.get l y = Some y' ->
-        post t m (map.put l x y')
+        post k t m (map.put l x y')
              (addMetricLoads 1
              (addMetricInstructions 1 mc)) ->
-        exec (SSet x y) t m l mc post
-    | if_true: forall t m l mc cond  bThen bElse post,
+        exec (SSet x y) k t m l mc post
+    | if_true: forall k t m l mc cond  bThen bElse post,
         eval_bcond l cond = Some true ->
-        exec bThen t m l
+        exec bThen (leak_bool true :: k) t m l
              (addMetricLoads 2
              (addMetricInstructions 2
              (addMetricJumps 1 mc))) post ->
-        exec (SIf cond bThen bElse) t m l mc post
-    | if_false: forall t m l mc cond bThen bElse post,
+        exec (SIf cond bThen bElse) k t m l mc post
+    | if_false: forall k t m l mc cond bThen bElse post,
         eval_bcond l cond = Some false ->
-        exec bElse t m l
+        exec bElse (leak_bool false :: k) t m l
              (addMetricLoads 2
              (addMetricInstructions 2
              (addMetricJumps 1 mc))) post ->
-        exec (SIf cond bThen bElse) t m l mc post
-    | loop: forall t m l mc cond body1 body2 mid1 mid2 post,
+        exec (SIf cond bThen bElse) k t m l mc post
+    | loop: forall k t m l mc cond body1 body2 mid1 mid2 post,
         (* This case is carefully crafted in such a way that recursive uses of exec
          only appear under forall and ->, but not under exists, /\, \/, to make sure the
          auto-generated induction principle contains an IH for all recursive uses. *)
-        exec body1 t m l mc mid1 ->
-        (forall t' m' l' mc',
-            mid1 t' m' l' mc' ->
+        exec body1 k t m l mc mid1 ->
+        (forall k' t' m' l' mc',
+            mid1 k' t' m' l' mc' ->
             eval_bcond l' cond <> None) ->
-        (forall t' m' l' mc',
-            mid1 t' m' l' mc' ->
+        (forall k' t' m' l' mc',
+            mid1 k' t' m' l' mc' ->
             eval_bcond l' cond = Some false ->
-            post t' m' l'
+            post (leak_bool false :: k') t' m' l'
                  (addMetricLoads 1
                  (addMetricInstructions 1
                  (addMetricJumps 1 mc')))) ->
-        (forall t' m' l' mc',
-            mid1 t' m' l' mc' ->
+        (forall k' t' m' l' mc',
+            mid1 k' t' m' l' mc' ->
             eval_bcond l' cond = Some true ->
-            exec body2 t' m' l' mc' mid2) ->
-        (forall t'' m'' l'' mc'',
-            mid2 t'' m'' l'' mc'' ->
-            exec (SLoop body1 cond body2) t'' m'' l''
+            exec body2 (leak_bool true :: k') t' m' l' mc' mid2) ->
+        (forall k'' t'' m'' l'' mc'',
+            mid2 k'' t'' m'' l'' mc'' ->
+            exec (SLoop body1 cond body2) k'' t'' m'' l''
                  (addMetricLoads 2
                  (addMetricInstructions 2
                  (addMetricJumps 1 mc''))) post) ->
-        exec (SLoop body1 cond body2) t m l mc post
-    | seq: forall t m l mc s1 s2 mid post,
-        exec s1 t m l mc mid ->
-        (forall t' m' l' mc', mid t' m' l' mc' -> exec s2 t' m' l' mc' post) ->
-        exec (SSeq s1 s2) t m l mc post
-    | skip: forall t m l mc post,
-        post t m l mc ->
-        exec SSkip t m l mc post.
+        exec (SLoop body1 cond body2) k t m l mc post
+    | seq: forall k t m l mc s1 s2 mid post,
+        exec s1 k t m l mc mid ->
+        (forall k' t' m' l' mc', mid k' t' m' l' mc' -> exec s2 k' t' m' l' mc' post) ->
+        exec (SSeq s1 s2) k t m l mc post
+    | skip: forall k t m l mc post,
+        post k t m l mc ->
+        exec SSkip k t m l mc post.
 
   End FlatImpExec.
 End exec.
