compiler/src/compiler/ExprImp.v
@@ -22,7 +22,6 @@ Section ExprImp1.
   Context {locals: map.map String.string word}.
   Context {env: map.map String.string (list String.string * list String.string * cmd)}.
   Context {ext_spec: ExtSpec}.
-  Context {leak_ext: LeakExt}.
 
   Notation var := String.string (only parsing).
   Notation func := String.string (only parsing).
@@ -380,7 +379,6 @@ Section ExprImp2.
   Context {locals: map.map String.string word}.
   Context {env: map.map String.string (list String.string * list String.string * cmd)}.
   Context {ext_spec: ExtSpec}.
-  Context {leak_ext: LeakExt}.
 
   Notation var := String.string (only parsing).
   Notation func := String.string (only parsing).
